Demo.v
@@ -168,8 +168,34 @@ Parameter bbb: bool.
 
 Quote Definition two_arg_fun_app_syn' := ((fun (x : nat) (_ : bool) => x) 1 bbb).
 
+Example two_arg_fun_eval : expr_eval_i 10 Σ [] (indexify [] [| {two_arg_fun_syn} Z true |]) =
+                           Ok (vConstr Nat "Z" []).
+Proof. compute. reflexivity. Qed.
+
+Example two_arg_fun_eval_named : expr_eval_n 10 Σ [] ([| {two_arg_fun_syn} Z true |]) =
+                           Ok (vConstr Nat "Z" []).
+Proof. compute. reflexivity. Qed.
+
+
+Compute expr_eval_i 10 Σ [] (indexify []   [| {plus_syn} 1 ({plus_syn} 1 1) |]).
+
+Compute expr_eval_i 10 Σ
+        ([(x, vClos [] y cmLam (tyInd Nat) (tyInd Nat) ([| \x : Nat -> ^0 |]));
+         (y,vConstr Nat "Z" []); (z,two)])
+        ([| ^0 ^1 ^2 |]).
+
+Compute expr_eval_n 10 Σ
+        ([(x, vClos [] y cmLam (tyInd Nat) (tyInd Nat) ([| \x : Nat -> x |]));
+         (y,vConstr Nat "Z" []); (z,two)])
+        ([| x y z |]).
+
+
+(* This example fails due to the bug in the new implementation of the interpreter *)
+Example one_plus_one_two : expr_eval_i 10 Σ [] (indexify [] one_plus_one) = Ok two.
+Proof. compute. reflexivity. Abort.
+
 Example one_plus_one_two : expr_eval_n 10 Σ [] one_plus_one = Ok two.
-Proof. reflexivity. Qed.
+Proof. compute. reflexivity. Qed.
 
 Definition plus_syn' :=
   [| \x : Nat ->
@@ -216,19 +242,25 @@ Definition id_rec :=
 
 Compute (expr_eval_n 20 Σ [] [| {id_rec} (Suc (Suc (Suc 1))) |]).
 Compute (expr_eval_i 20 Σ [] (indexify [] [| {id_rec} (Suc (Suc (Suc 1))) |])).
+Compute (from_nested_app [| {id_rec} (Suc (Suc (Suc 1))) |]).
+Compute (args_nested_app [| {id_rec} (Suc (Suc (Suc 1))) |]).
+
+Compute (expr_eval_i 20 Σ []
+                     (indexify []
+                               [| (\x : Nat -> \y : Nat -> x) Z Z |])).
 
 Example id_rec_named_and_indexed :
   let arg := [| Suc (Suc (Suc 1)) |] in
   expr_eval_n 20 Σ [] [| {id_rec} {arg} |] =
   expr_eval_i 20 Σ [] (indexify [] [| {id_rec} {arg} |]).
-Proof. reflexivity. Qed.
+Proof. compute. reflexivity. Qed.
 
-Example plus_named_and_indexed :
-  let two := [| (Suc 1)|] in
-  let three := [| Suc {two} |] in
-  expr_eval_n 20 Σ [] [| ({plus_syn} {two}) {three} |] =
-  expr_eval_i 20 Σ [] (indexify [] [| ({plus_syn} {two}) {three} |]).
-Proof. reflexivity. Qed.
+(* Example plus_named_and_indexed : *)
+(*   let two := [| (Suc 1)|] in *)
+(*   let three := [| Suc {two} |] in *)
+(*   expr_eval_n 20 Σ [] [| ({plus_syn} {two}) {three} |] = *)
+(*   expr_eval_i 20 Σ [] (indexify [] [| ({plus_syn} {two}) {three} |]). *)
+(* Proof. reflexivity. Qed. *)
 
 Compute ( v <- (expr_eval_i 10 Σ [] (indexify [] [| {one_plus_one} |]));;
           ret (from_val v)).
